\documentclass[a4paper,12pt]{extarticle}
\usepackage{geometry,microtype,mathtools,amsthm,amssymb}
\usepackage[utf8]{inputenc}
\usepackage[font=small,labelfont=bf]{caption}
\theoremstyle{definition}
\newtheorem{definition}{Definition} \newtheorem{theorem}{Theorem} \newtheorem{corollary}{Corollary}[theorem] \newtheorem*{remark}{Remark}
\newcommand{\R}{\mathbb{R}} \newcommand{\Q}{\mathbb{Q}} \newcommand{\Z}{\mathbb{Z}} \newcommand{\N}{\mathbb{N}} \newcommand{\myskip}{\par\null\par} \renewcommand\qedsymbol{QED} \renewcommand{\leq}{\leqslant}\renewcommand{\geq}{\geqslant}
\title{Math 431 Homework 10} 
\author{Theo Koss}
\date{November 2022}
\begin{document}
\maketitle
\section{Section 8.6}
\begin{itemize}
    \item Problem 15(b): $$H = \begin{pmatrix}
    0 & 0 & 1 & 0 & 0 & 1 & 0 & 0 & 0\\
    1 & 1 & 0 & 1 & 0 & 0 & 1 & 0 & 0\\
    0 & 1 & 0 & 1 & 0 & 0 & 0 & 1 & 0\\
    1 & 1 & 0 & 0 & 1 & 0 & 0 & 0 & 1\\
    \end{pmatrix}$$ $$G = \begin{pmatrix}
    1 & 0 & 0 & 0 & 0 \\
    0 & 1 & 0 & 0 & 0 \\
    0 & 0 & 1 & 0 & 0 \\
    0 & 0 & 0 & 1 & 0 \\
    0 & 0 & 0 & 0 & 1 \\
    0 & 0 & 1 & 0 & 0 \\
    1 & 1 & 0 & 1 & 0 \\
    0 & 1 & 0 & 1 & 0 \\
    1 & 1 & 0 & 0 & 1 \\
    \end{pmatrix}$$ $$C = \{0, (100000101), (010000111), (001001000), (000100110), (000010001), (110000010),$$ $$ (101001101), (100100011), (100010100), (011001111), (010100001), (010010110),$$ $$(001101110), (001011001), (000110111)\}$$
    \begin{table}[h]
        \centering
        \begin{tabular}{c|c}
            Syndrome & Coset leader \\
            \hline
        \end{tabular}
        \caption{Decoding Table}
        \label{tab:my_label}
    \end{table}
\end{itemize}
\section{Section 9.4}
\begin{itemize}
    \item Problem 9: \begin{itemize}
        \item Associative: \begin{align*}
        (a*b)*c&=(a+b+ab)*c\\
        &=a+c+ac+b+c+bc+ab+c+abc\\
        a*(b*c)&=a*(b+c+bc)\\
        &=a+b+ab+a+c+ac+a+bc+abc
        \end{align*} By commutativity of $+$, they are equal
        \item Identity: $0\in G$, since $a*0=0*a=a+0+0$.
        \item Inverses: Consider $a\in G$, then the inverse is $-\frac{a}{a+1}\in G$.
    \end{itemize}
    Consider an isomorphism $\phi: G\to H$, defined as $\phi(a)=a+1$. This is clearly one to one and onto. Then $\phi(a*b)=\phi(a)\cdot\phi(b)$ since \begin{align*}
        \phi(a*b)&=a*b+1\\
        &=(a+1)(b+1)-1+1\\
        &=(a+1)(b+1)\\
        &=\phi(a)\cdot\phi(b)
    \end{align*} As required. Thus, $(G,*)\cong(H,\cdot)$s
\end{itemize}
\end{document}