\documentclass[hidelinks,12pt]{article}
\usepackage[utf8]{inputenc}
\usepackage[table,xcdraw]{xcolor}
\usepackage{mathtools}
\usepackage{amsthm}
\usepackage{amsmath}
\usepackage{amsfonts}
\usepackage{amssymb}
\usepackage{centernot}
\usepackage{marvosym}
\usepackage{enumitem}
\usepackage{hyperref}
\setcounter{tocdepth}{1}
\usepackage{chngcntr}
\counterwithin*{equation}{section}
\counterwithin*{equation}{subsection}
\let\marvosymLightning\Lightning
\newtheorem{theorem}{Theorem}
\newtheorem{corollary}{Corollary}[theorem]
\newtheorem*{remark}{Remark}
\renewcommand\qedsymbol{QED}
\newcommand{\C}{\mathbb{C}}
\newcommand{\R}{\mathbb{R}}
\newcommand{\N}{\mathbb{N}}
\newcommand{\Z}{\mathbb{Z}}
\newcommand{\Q}{\mathbb{Q}}
\newcommand{\divby}{%
  \mathrel{\text{\vbox{\baselineskip.65ex\lineskiplimit0pt\hbox{.}\hbox{.}\hbox{.}}}}%
  }
\newcommand{\notdivby}{\centernot\divby}
\title{\scalebox{2}{Math 531 Homework 9}}
\author{\scalebox{1.5}{Theo Koss}}
\date{April 2021}
\begin{document}
\maketitle
\section{Section 5.4}
\begin{itemize}
\item Problem 2: Show that the associative and commutative laws hold for addition in $\Q(D)$.\begin{proof}\begin{enumerate}[label=(\alph*)]
    \item Associative: Let $$x=a_1+b_1D$$ $$y=a_2+b_2D$$ $$z=a_3+b_3D$$ N2S: $(x+y)+z=x+(y+z)$. $$(x+y)+z=(a_1+b_1D+a_2+b_2D)+a_3+b_3D$$ $$=((a_1+a_2)+(b_1+b_2)D)+a_3+b_3D$$ $$=(a_1+a_2)+a_3+(b_1+b_2)D+b_3D$$ $$=a_1+(a_2+a_3)+((b_1+b_2)+b_3)D$$ $$=a_1+(a_2+a_3)+b_1D+(b_2+b_3)D$$ $$=a_1+b_1D+[(a_2+a_3)+(b_2+b_3)D]$$ $$=a_1+b_1D+[a_2+b_2D+a_3+b_3D]$$ $$=x+(y+z)$$ As required.
    \item Commutative: Let $$x=a_1+b_1D$$ $$y=a_2+b_2D$$ $$x+y=(a_1+b_1D)+(a_2+b_2D)$$ $$=(a_1+a_2)+(b_1+b_2)D$$ $$=(a_2+a_1)+(b_2+b_1)D$$ $$=a_2+a_1+b_2D+b_1D$$ $$a_2+b_2D+a_1+b_1D$$ $$=y+x$$ As required.
 \end{enumerate}
\end{proof}
\item Problem 3: Show that the associative and commutative laws hold for multiplication in $\Q(D)$.\begin{proof}\begin{enumerate}[label=(\alph*)]
\item Associative: Let $$x=a_1+b_1D$$ $$y=a_2+b_2D$$ $$z=a_3+b_3D$$ N2S: $x\cdot (y\cdot z)=(x\cdot y)\cdot z$. $$x\cdot (y\cdot z)=(a_1+b_1D)\cdot((a_2+b_2D)\cdot(a_3+b_3D))$$ $$=(a_1+b_1D)\cdot((a_2a_3-b_2b_3)+(a_2b_3+b_2a_3)D)$$ $$=(a_1(a_2a_3-b_2b_3)-b_1(a_2b_3+b_2a_3))+(a_1(a_2b_3+b_2a_3)+b_1(a_2a_3-b_2b_3))D$$ $$=(a_1a_2a_3-a_1b_2b_3-b_1a_2b_3-b_1b_2a_3)+(a_1a_2b_3+a_1b_2a_3+b_1a_2a_3-b_1b_2b_3)D$$ 
$$(x\cdot y)\cdot z=((a_1a_2-b_1b_2)+(a_1b_2+b_1a_2)D)\cdot(a_3+b_3D)$$ $$=(a_1a_2a_3-a_1b_2b_3-b_1a_2b_3-b_1b_2a_3)+(a_1a_2b_3+a_1b_2a_3+b_1a_2a_3-b_1b_2b_3)D$$ $$=x\cdot (y\cdot z)$$ As required, therefore multiplication is associative in $\Q(D)$.

\item Commutative: Let $$x=a_1+b_1D$$ $$y=a_2+b_2D$$ $$x\cdot y=(a_1+b_1D)\cdot(a_2+b_2D)=(a_1a_2-b_1b_2)+(a_1b_2+b_1a_2)D$$ $$y\cdot x=(a_2+b_2D)\cdot(a_1+b_1D)=(a_2a_1-b_2b_1)+(b_2a_1+a_2b_1)D$$ $$=(a_1a_2-b_1b_2)+(a_1b_2+b_1a_2)D$$
$$\therefore x\cdot y=y\cdot x$$ Thus multiplication is commutative in $\Q(D)$.
\end{enumerate}
\end{proof}
\end{itemize}
\end{document}