\documentclass[12pt]{article}
\usepackage[utf8]{inputenc}
\usepackage{mathtools}
\usepackage{amsmath}
\usepackage{amsfonts}
\usepackage{amssymb}
\usepackage{amsthm}
\usepackage{centernot}
\newcommand{\notequiv}{\centernot\equiv}
\newcommand{\N}{\mathbb{N}}
\newcommand{\Z}{\mathbb{Z}}
\newtheorem{theorem}{Theorem}
\newcommand{\divby}{%
  \mathrel{\text{\vbox{\baselineskip.65ex\lineskiplimit0pt\hbox{.}\hbox{.}\hbox{.}}}}%
  }
\newcommand{\notdivby}{\centernot\divby}
\renewcommand\qedsymbol{QED}
\title{\scalebox{2}{Math 341 Exam 1}}
\author{\scalebox{1.5}{Theo Koss}}
\date{September 2020}
\begin{document}
\maketitle
\section{Problem 2}
Prove by induction: if $a\geq-1$, then, $(1+a)^n\geq1+na$ for all $n\geq0$.
\begin{proof}
\emph{Basis}: Check for $n=1$: $1+a\geq1+a$.\newline \emph{Inductive step}: \newline Assume the formula holds for $n=k$, so $(1+a)^k\geq(1+ka), a\geq-1$ We must show it holds for $n=k+1$, that is: $$(1+a)^{k+1}\geq(1+(k+1)a)$$ Simplifying:$$(1+a)\cdot(1+a)^k\geq(1+a(k+1))$$ Using our assumption:$$(1+a)^k\cdot(1+a)\geq(1+a(k+1))\cdot(1+a)$$ Thus:$$(1+a)^{k+1}\geq(1+(k+1)a)\cdot(1+a)\Longrightarrow(1+a)^{k+1}\geq(1+(k+1)a)$$ As required.
\end{proof}
\end{document}